ironfleet/src/Dafny/Distributed/Common/Framework/Main.s.dfy
@@ -52,6 +52,7 @@ lemma RefinementProof(config:DS_s.H_s.ConcreteConfiguration, db:seq<DS_State>) r
   requires |db| > 0
   requires DS_Init(db[0], config)
   requires forall i {:trigger DS_Next(db[i], db[i+1])} :: 0 <= i < |db| - 1 ==> DS_Next(db[i], db[i+1])
+  requires forall i :: 0 <= i < |db| ==> forall id :: id in db[i].servers ==> DS_s.H_s.HostGroupSize(db[i].servers[id])
   ensures  |db| == |sb|
   ensures  Service_Init(sb[0], Collections__Maps2_s.mapdomain(db[0].servers))
   ensures  forall i {:trigger Service_Next(sb[i], sb[i+1])} :: 0 <= i < |sb| - 1 ==> sb[i] == sb[i+1] || Service_Next(sb[i], sb[i+1])
