ironfleet/src/Dafny/Distributed/Services/RSL/Main.i.dfy
@@ -103,13 +103,15 @@ function AbstractifyConcreteEnvironment(ds_env:LEnvironment<EndPoint,seq<byte>>)
 
 function AbstractifyConcreteReplicas(replicas:map<EndPoint,HostState>, replica_order:seq<EndPoint>) : seq<LScheduler>
   requires forall r :: r in replica_order ==> r in replicas
+  requires forall i :: 0 <= i < |replica_order| ==>
+             |replicas[replica_order[i]].groups| == 1
   ensures  |AbstractifyConcreteReplicas(replicas, replica_order)| == |replica_order|
   ensures  forall i :: 0 <= i < |replica_order| ==>
-             AbstractifyConcreteReplicas(replicas, replica_order)[i] == replicas[replica_order[i]].csched.sched
+             AbstractifyConcreteReplicas(replicas, replica_order)[i] == replicas[replica_order[i]].groups[0].sched
 {
   if replica_order == [] then []
   else
-    [replicas[replica_order[0]].csched.sched] + AbstractifyConcreteReplicas(replicas, replica_order[1..])
+    [replicas[replica_order[0]].groups[0].sched] + AbstractifyConcreteReplicas(replicas, replica_order[1..])
 }
 
 function AbstractifyConcreteClients(clients:set<EndPoint>) : set<NodeIdentity>
@@ -126,6 +128,8 @@ predicate DsStateIsAbstractable(ds:DS_State)
 
 function AbstractifyDsState(ds:DS_State) : RslState
   requires DsStateIsAbstractable(ds)
+  requires forall i :: 0 <= i < |ds.config.config.replica_ids| ==>
+             |ds.servers[ds.config.config.replica_ids[i]].groups| == 1
 {
   RslState(AbstractifyConstantsStateToLConstants(ds.config),
            AbstractifyConcreteEnvironment(ds.environment),
@@ -203,12 +207,15 @@ lemma {:timeLimitMultiplier 2} lemma_DsConstantsAllConsistent(config:ConcreteCon
   requires IsValidBehavior(config, db)
   requires 0 <= i < |db|
   requires id in db[i].servers
+  requires forall j :: 0 <= j < |db| ==>
+            forall k :: k in db[j].servers ==>
+              DS_s.H_s.HostGroupSize(db[j].servers[k]);
   ensures  db[i].config == config
-  ensures  db[i].servers[id].csched.sched.replica.constants.all == AbstractifyConstantsStateToLConstants(config)
-  ensures  db[i].servers[id].csched.sched.replica.proposer.constants.all == AbstractifyConstantsStateToLConstants(config)
-  ensures  db[i].servers[id].csched.sched.replica.acceptor.constants.all == AbstractifyConstantsStateToLConstants(config)
-  ensures  db[i].servers[id].csched.sched.replica.learner.constants.all == AbstractifyConstantsStateToLConstants(config)
-  ensures  db[i].servers[id].csched.sched.replica.executor.constants.all == AbstractifyConstantsStateToLConstants(config)
+  ensures  db[i].servers[id].groups[0].sched.replica.constants.all == AbstractifyConstantsStateToLConstants(config)
+  ensures  db[i].servers[id].groups[0].sched.replica.proposer.constants.all == AbstractifyConstantsStateToLConstants(config)
+  ensures  db[i].servers[id].groups[0].sched.replica.acceptor.constants.all == AbstractifyConstantsStateToLConstants(config)
+  ensures  db[i].servers[id].groups[0].sched.replica.learner.constants.all == AbstractifyConstantsStateToLConstants(config)
+  ensures  db[i].servers[id].groups[0].sched.replica.executor.constants.all == AbstractifyConstantsStateToLConstants(config)
 {
   if i == 0
   {
@@ -224,8 +231,8 @@ lemma {:timeLimitMultiplier 2} lemma_DsConstantsAllConsistent(config:ConcreteCon
 
   lemma_DsConstantsAllConsistent(config, db, i-1, id);
 
-  var s := db[i-1].servers[id].csched.sched;
-  var s' := db[i].servers[id].csched.sched;
+  var s := db[i-1].servers[id].groups[0].sched;
+  var s' := db[i].servers[id].groups[0].sched;
 
   if s' == s
   {
@@ -547,8 +554,11 @@ lemma lemma_IgnoringCertainMessageTypesFromNonServerIsLSchedulerNext(
   requires 0 <= i < |db| - 1
   requires id in db[i].servers
   requires id in db[i+1].servers
-  requires s == db[i].servers[id].csched.sched
-  requires s' == db[i+1].servers[id].csched.sched
+  requires forall j :: 0 <= j < |db| ==>
+            forall id :: id in db[j].servers ==>
+              DS_s.H_s.HostGroupSize(db[j].servers[id]);
+  requires s == db[i].servers[id].groups[0].sched
+  requires s' == db[i+1].servers[id].groups[0].sched
   requires s.nextActionIndex == 0
   requires s' == s.(nextActionIndex := (s.nextActionIndex + 1) % LReplicaNumActions())
   requires |ios| == 1
@@ -579,11 +589,14 @@ lemma lemma_HostNextIgnoreUnsendableIsLSchedulerNext(
   requires db[i].environment.nextStep == LEnvStepHostIos(id, ios)
   requires id in db[i].servers
   requires id in db[i+1].servers
+  requires forall j :: 0 <= j < |db| ==>
+            forall id :: id in db[j].servers ==>
+              DS_s.H_s.HostGroupSize(db[j].servers[id]);
   requires LEnvironment_Next(db[i].environment, db[i+1].environment)
   requires ValidPhysicalEnvironmentStep(db[i].environment.nextStep)
-  requires HostNextIgnoreUnsendable(db[i].servers[id].csched.sched, db[i+1].servers[id].csched.sched, ios)
+  requires HostNextIgnoreUnsendable(db[i].servers[id].groups[0].sched, db[i+1].servers[id].groups[0].sched, ios)
   requires NetEventLogIsAbstractable(ios)
-  ensures  LSchedulerNext(db[i].servers[id].csched.sched, db[i+1].servers[id].csched.sched, AbstractifyRawLogToIos(ios))
+  ensures  LSchedulerNext(db[i].servers[id].groups[0].sched, db[i+1].servers[id].groups[0].sched, AbstractifyRawLogToIos(ios))
 {
   var p := ios[0].r;
   var rp := AbstractifyNetPacketToRslPacket(p);
@@ -607,8 +620,8 @@ lemma lemma_HostNextIgnoreUnsendableIsLSchedulerNext(
   assert |rios| == 1;
   assert rios[0].r == rp;
 
-  var s := db[i].servers[id].csched.sched;
-  var s' := db[i+1].servers[id].csched.sched;
+  var s := db[i].servers[id].groups[0].sched;
+  var s' := db[i+1].servers[id].groups[0].sched;
 
   assert s.nextActionIndex == 0;
   calc {
@@ -646,6 +659,9 @@ lemma {:timeLimitMultiplier 2} lemma_RslNext(
   requires 0 <= i < |db| - 1
   requires DsStateIsAbstractable(db[i])
   requires DsStateIsAbstractable(db[i+1])
+  requires forall j :: 0 <= j < |db| ==>
+            forall id :: id in db[j].servers ==>
+              DS_s.H_s.HostGroupSize(db[j].servers[id]);
   requires ls  == AbstractifyDsState(db[i])
   requires ls' == AbstractifyDsState(db[i+1])
   requires forall id :: id in db[i].servers ==> id in db[i].config.config.replica_ids
@@ -679,13 +695,15 @@ lemma {:timeLimitMultiplier 2} lemma_RslNext(
 
   assert ls.environment.nextStep == LEnvStepHostIos(id, r_ios);
 
-  assert || LSchedulerNext(ds.servers[id].csched.sched, ds'.servers[id].csched.sched, r_ios)
-         || HostNextIgnoreUnsendable(ds.servers[id].csched.sched, ds'.servers[id].csched.sched, ios);
-  if HostNextIgnoreUnsendable(ds.servers[id].csched.sched, ds'.servers[id].csched.sched, ios)
+  assert (id in ds.servers) && (id in ds'.servers) && (|ds.servers[id].groups| == 1) && (|ds'.servers[id].groups| == 1);
+
+  assert || LSchedulerNext(ds.servers[id].groups[0].sched, ds'.servers[id].groups[0].sched, r_ios)
+         || HostNextIgnoreUnsendable(ds.servers[id].groups[0].sched, ds'.servers[id].groups[0].sched, ios);
+  if HostNextIgnoreUnsendable(ds.servers[id].groups[0].sched, ds'.servers[id].groups[0].sched, ios)
   {
     lemma_HostNextIgnoreUnsendableIsLSchedulerNext(config, db, i, id, ios);
   }
-  assert LSchedulerNext(ds.servers[id].csched.sched, ds'.servers[id].csched.sched, r_ios);
+  assert LSchedulerNext(ds.servers[id].groups[0].sched, ds'.servers[id].groups[0].sched, r_ios);
 
   assert LEnvironment_Next(ds.environment, ds'.environment);
   lemma_LEnvironmentNextHost(ds.environment, ls.environment, ds'.environment, ls'.environment);
@@ -706,6 +724,9 @@ lemma lemma_GetImplBehaviorRefinement(config:ConcreteConfiguration, db:seq<DS_St
   returns (protocol_behavior:seq<RslState>, c:LConstants)
   requires IsValidBehavior(config, db)
   requires LEnvStepIsAbstractable(last(db).environment.nextStep)
+  requires forall i :: 0 <= i < |db| ==>
+            forall id :: id in db[i].servers ==>
+              DS_s.H_s.HostGroupSize(db[i].servers[id]);
   ensures |protocol_behavior| == |db|
   ensures protocol_behavior[0].constants == AbstractifyConstantsStateToLConstants(config)
   ensures RslInit(c, protocol_behavior[0])
@@ -939,6 +960,9 @@ lemma{:timeLimitMultiplier 4} lemma_RefinementProofForFixedBehavior(config:Concr
   returns (sb:seq<ServiceState>)
   requires IsValidBehavior(config, db)
   requires last(db).environment.nextStep.LEnvStepStutter?
+  requires forall i :: 0 <= i < |db| ==>
+            forall id :: id in db[i].servers ==>
+              DS_s.H_s.HostGroupSize(db[i].servers[id]);
   ensures  |db| == |sb|
   ensures  Service_Init(sb[0], mapdomain(db[0].servers))
   ensures  forall i {:trigger Service_Next(sb[i], sb[i+1])} :: 0 <= i < |sb| - 1 ==> sb[i] == sb[i+1] || Service_Next(sb[i], sb[i+1])
@@ -1012,6 +1036,7 @@ lemma{:timeLimitMultiplier 4} lemma_RefinementProofForFixedBehavior(config:Concr
 
 lemma lemma_FixFinalEnvStep(config:ConcreteConfiguration, db:seq<DS_State>) returns (db':seq<DS_State>)
   requires IsValidBehavior(config, db)
+  requires  forall i :: 0 <= i < |db| ==> forall id :: id in db[i].servers ==> DS_s.H_s.HostGroupSize(db[i].servers[id])
   ensures  |db'| == |db|
   ensures  DS_Init(db'[0], config)
   ensures  forall i {:trigger DS_Next(db'[i], db'[i+1])} :: 0 <= i < |db'| - 1 ==> DS_Next(db'[i], db'[i+1])
@@ -1019,6 +1044,7 @@ lemma lemma_FixFinalEnvStep(config:ConcreteConfiguration, db:seq<DS_State>) retu
   ensures  forall i :: 0 <= i < |db'| - 1 ==> db'[i] == db[i]
   ensures  last(db') == last(db).(environment := last(db').environment)
   ensures  last(db').environment == last(db).environment.(nextStep := LEnvStepStutter())
+  ensures  forall i :: 0 <= i < |db'| ==> forall id :: id in db'[i].servers ==> DS_s.H_s.HostGroupSize(db'[i].servers[id])
 {
   var sz := |db|;
   db' := all_but_last(db) + [last(db).(environment := last(db).environment.(nextStep := LEnvStepStutter()))];
@@ -1036,7 +1062,13 @@ lemma lemma_FixFinalEnvStep(config:ConcreteConfiguration, db:seq<DS_State>) retu
 
 lemma RefinementProof(config:DS_s.H_s.ConcreteConfiguration, db:seq<DS_State>) returns (sb:seq<ServiceState>)
 {
+  assert forall i :: 0 <= i < |db| ==>
+            forall id :: id in db[i].servers ==>
+              DS_s.H_s.HostGroupSize(db[i].servers[id]);
   var db' := lemma_FixFinalEnvStep(config, db);
+  assert forall i :: 0 <= i < |db'| ==>
+            forall id :: id in db'[i].servers ==>
+              DS_s.H_s.HostGroupSize(db'[i].servers[id]);
   sb := lemma_RefinementProofForFixedBehavior(config, db');
 }
 
